\chapter{Grammar}

\section{Context Free Grammar}

  A context free grammar has four components

  \begin{itemize}
    \item A set of \textbf{terminal symbols} representing individual tokens
    \begin{equation*}
      prep
    \end{equation*}
    \begin{itemize}
      \item Lower case
    \end{itemize}

    \item A set of \textbf{non-terminal symbols} representing sytnax trees
    \begin{equation*}
      N
    \end{equation*}
    \begin{itemize}
      \item Upper case
    \end{itemize}

    \item A set of \textbf{productions}, each mapping a non terminal symbol
    to string of terminal and non-terminal symbols
    \begin{align*}
      N &\to prep \text{ } N \\
      &\left| N \text{ } prep \right.
    \end{align*}

    \item A designated non terminal symbol called the \textbf{start symbol}
    \begin{equation}
      S \to N
    \end{equation}
  \end{itemize}

  \subsection{Properties of Grammar}

    \begin{itemize}
      \item \textbf{Epsilon Production}: a production of the form
      \begin{equation*}
        E \to \epsilon
      \end{equation*}
      where $ \epsilon $ represents the empty string

      \begin{itemize}
        \item A symbol \textbf{can be nothing, or optional (represented using
        $ \epsilon $)}
      \end{itemize}

      \item \textbf{Right Linear}: grammars where all the productions have the
      form
      \begin{align*}
        E &\to x F \\
        E &\to x
      \end{align*}

      \begin{itemize}
        \item Corresponds to \textbf{regular languages}
      \end{itemize}

      This is not a right linear grammar
      \begin{align*}
        S_{0} &\to c S_{1} c S_{2} c
      \end{align*}

      \item \textbf{Left Recursive}: a production like
      \begin{equation*}
        E \to E + X
      \end{equation*}

      \item \textbf{Ambiguous}: more than one parse tree is possible for a
      specific sentence
    \end{itemize}

  \subsection{Dangling Else Problem}

    \begin{align*}
      E &\to \text{ if } E \text{ then } E \text{ else } E \\
      E &\to \text{ if } E \text{ then } E \\
      E &\to \text{ whatever}
    \end{align*}

    \paragraph{Solution}
    \begin{enumerate}
      \item Use recursion only one one side; ex. left-recursive
      \item Divide the grammar into multiple rules, and then put highest
      precedence rules lower in the new grammar
    \end{enumerate}

\section{LL Grammar}

  \begin{definition}
    A $ \LL $ grammar is a context-free grammar that can be used by a LL parser
  \end{definition}

  \subsection{LL(k) Grammar}

    \begin{definition}
      A $ \LL\left( k \right) $ grammar is a LL grammar where the parser can
      peek at most $ k $ tokens; the parser can use the peeks to make a
      deterministic decision, without context (aka. backtracking)
    \end{definition}

\section{Sets}
  \subsection{FIRST Set}

    \begin{definition}
      \textbf{FIRST Set}: the set of terminal symbols that we are going to see
      first
    \end{definition}

    \subsection{Finding FIRST}

      For each symbol $ X $

      \begin{enumerate}
        \item If $ X $ is a terminal, then $ \FIRST\left( X \right) = { X } $
        \item If there is a production $ X \to \epsilon $, then add $ \epsilon $
        to $ \FIRST\left( X \right) $
        \item If there is a production $ X \to Y_{1} ... Y_{n} $, then add
        $ \FIRST\left( Y_{1} ... Y_{n} \right) $ to $ \FIRST\left( X \right) $
        \begin{enumerate}
          \item If $ \FIRST\left( Y_{1} \right) $ does not contain $ \epsilon $,
          then:
          \begin{equation}
            \FIRST\left( Y_{1} ... Y_{n} \right) = \FIRST\left( Y_{1} \right)
          \end{equation}

          \item Otherwise
          \begin{equation}
            \FIRST\left( Y_{1} ... Y_{n} \right) =
              \frac{\FIRST\left( Y_{1} \right)}{\epsilon} \cup
              \FIRST\left( Y_{2} ... Y_{n} \right)
          \end{equation}

          \item If all of $ Y_{1} ... Y_{n} $ have $ \epsilon $, then add
          $ \epsilon $ to $ \FIRST\left( X \right) $
        \end{enumerate}
      \end{enumerate}

  \subsection{FOLLOW Set}

    \begin{definition}
      \textbf{FOLLOW Set}: A list of symbols that can occur after parsing
      non-terminals
    \end{definition}

    \subsection{Finding FOLLOW}

      $ \alpha, \beta $ represents terminal and nonterminal symbols

      \begin{enumerate}
        \item Put $ \$ $ in $ \FOLLOW\left( S \right) $, where $ S $ is the start
        symbol; $ \$ $ represents end of input
        \item If there is a production $ X \to \alpha Y \beta $, then add
        $ \FIRST\left( \beta \right) $ to $ \FOLLOW\left( Y \right) $
        \item If there is a production $ X \to \alpha Y $, or if there is \ul{a
        production $ X \to \alpha Y \beta $, where
        $ \epsilon \in \FIRST\left( \beta \right) $} then add
        $ \FOLLOW\left( X \right) $ to $ \FOLLOW\left( Y \right) $
      \end{enumerate}

  \subsection{Epsilon Productions}

    Epsilon productions introduces ambiguity in the FOLLOW set

    \begin{align*}
      A &\to Bc | x \\
      B &\to c | \epsilon
    \end{align*}

    Solution, substitute certain productions

    \begin{align*}
      A &\to c A' | x \\
      A' &\to c | \epsilon
    \end{align*}

    Make sure to not introduce common prefixes

\section{Eliminate Left Recursion}
\label{section: grammar/eliminate left recursion}

  \begin{align*}
    E &\to Ea \\
    &\to i
  \end{align*}

  \begin{enumerate}
    \item Production of the form $ S \to \beta $ becomes $ S \to \beta S' $
    \item Production of the form $ S \to S \alpha $ becomes $ S' \to \alpha S' $
    \item Add $ S' \to \epsilon $
  \end{enumerate}

  \subsection{Mutual Recursion}

    \begin{align*}
      A &\to Ax | Bx \\
      B &\to Bx | Ax
    \end{align*}

    Inline either $ A $ or $ B $

\section{Eliminate Common Prefix}
\label{section: grammar/eliminate common prefix}

  Common prefixes introduce ambiguity in the FIRST set

  \begin{align*}
    A &\to \alpha \beta_{1} | \alpha \beta_{2}
  \end{align*}

  Extract the common part to get a new production

  \begin{align*}
    A &\to \alpha A' \\
    A' &\to \beta_{1} | \beta_{2}
  \end{align*}
