\chapter{Derivatives}

\begin{align}
  \frac{d}{dx} x^{a} &= a x^{a - 1} \\
  \frac{d}{dx} f\left( g \left( x \right) \right) &=
    f'\left( g\left( x \right) \right) g'\left( x \right) \\
\end{align}

\begin{align}
  \frac{d}{dx} e^{x} &= e^{x} \\
  \frac{d}{dx} e^{-x} &= e^{-x} \frac{d}{dx} \left( -x \right) = - e^{-x}
\end{align}

\begin{align*}
  \frac{d g\left( x \right)}{d f\left( x \right)}
    &= \frac{d g\left( x \right)}{dx} \frac{dx}{d f\left( x \right)} \\
    &= g'\left( x \right) \frac{1}{f'\left( x \right)} \\
    &= \frac{g'\left( x \right)}{f'\left( x \right)}
\end{align*}
